got rid of special types for OCaml instructions and programs; removed current proof to refactor high-level reasoning further

src/ocamlmm/OCamlToimm_s_prog.v
@@ -22,17 +22,16 @@ Remove Hints plus_n_O.
 
 
 Section OCaml_Program.
-  Definition Oinstlist := list Prog.Instr.t.
     
-  Definition Othread_execution (tid : thread_id) (insts : Oinstlist) (pe : execution) :=
+  Definition Othread_execution (tid : thread_id) (insts : list Prog.Instr.t) (pe : execution) :=
     exists s,
       ⟪ STEPS : (step tid)＊ (init insts) s ⟫ /\
       ⟪ TERMINAL : is_terminal s ⟫ /\
       ⟪ PEQ : s.(G) = pe ⟫.
 
-  Definition OProg := IdentMap.t Oinstlist.
+  Definition OCamlProgram (prog: Prog.Prog.t) := True. 
 
-  Definition Oprogram_execution (prog : OProg) (G : execution) :=
+  Definition Oprogram_execution prog (OPROG: OCamlProgram prog) (G : execution) :=
     (forall e (IN: G.(acts_set) e), is_init e \/ IdentMap.In (tid e) prog)
     /\ forall thread linstr (INTHREAD: IdentMap.find thread prog = Some linstr),
       exists pe, Othread_execution thread linstr pe
@@ -48,7 +47,7 @@ Section OCamlMM_TO_IMM_S_PROG.
   Proof.
   Admitted. 
 
-  Inductive is_thread_compiled : Oinstlist -> list Prog.Instr.t -> Prop :=
+  Inductive is_thread_compiled : list Prog.Instr.t -> list Prog.Instr.t -> Prop :=
   | compiled_empty: is_thread_compiled [] []
   | compiled_Rna lhs loc ro ri (rest: is_thread_compiled ro ri):
       let ld := (Instr.load Orlx lhs loc) in
@@ -74,7 +73,7 @@ Section OCamlMM_TO_IMM_S_PROG.
       is_thread_compiled (igt :: ro) (igt :: ri). 
   
 
-  Definition is_compiled (po: OProg) (pi: Prog.Prog.t) :=
+  Definition is_compiled (po: Prog.Prog.t) (pi: Prog.Prog.t) :=
     ⟪ SAME_THREADS: forall t_id, IdentMap.In t_id po <-> IdentMap.In t_id pi ⟫ /\
     forall thread to ti (TO: IdentMap.find thread po = Some to)
       (TI: IdentMap.find thread pi = Some ti),
@@ -114,177 +113,26 @@ Section OCamlMM_TO_IMM_S_PROG.
               GI.(lab) e = Aload true Osc loc val /\
               GO.(lab) w = Astore Xpln Osc loc val /\
               rmw_pair e w) in
-    ⟪OMM_SCALED: forall e (OMM_EVENT: E GO e), exists num, index e = 3 * num ⟫ /\
+    (* ⟪OMM_SCALED: forall e (OMM_EVENT: E GO e), exists num, index e = 3 * num ⟫ /\ *)
     ⟪ADD_EVENTS: E GI ≡₁ E GO ∪₁ Facq' ∪₁ Facqrel' ∪₁ R' ⟫ /\
     ⟪EXT_LABELS: wf_labels ⟫ /\
     ⟪NEW_RMW: GI.(rmw) ≡ fun r w => (E GI ∩₁ R GI ∩₁ Sc GI) r /\ (E GI ∩₁ W GI ∩₁ Sc GI) w /\ rmw_pair r w ⟫ /\
     ⟪SAME_CO: GI.(co) ≡ GO.(co)⟫ /\
     ⟪EXT_RF: GO.(rf) ⊆ GI.(rf)⟫. 
       
-  Variable ProgO: OProg.
-
-  Variable ProgI: Prog.Prog.t.
+  Variable ProgO ProgI: Prog.Prog.t.
   Hypothesis Compiled: is_compiled ProgI ProgO.
-
-  Definition compile_grouped EE shift event :=
-    Nat.eqb (Nat.modulo (index event) 3) 0 /\
-    EE (ThreadEvent (tid event) (index event + shift)). 
+  Hypothesis OCamlProgO: OCamlProgram ProgO. 
 
   Theorem compilation_correctness:
     forall (GI: execution) (WF: Wf GI) sc (ExecI: program_execution ProgI GI) 
-      (IPC: imm_s.imm_psc_consistent GI sc)
-      (IMM_SCALED: forall e (IMM_EVENT: E GI e), exists num,
-            ((set_compl (F GI ∪₁ dom_rel GI.(rmw))) e /\ index e = 3 * num) \/ 
-            (F GI e /\ index e = 3 * num - 2) \/
-            (dom_rel GI.(rmw) e /\ index e = 3 * num - 1)),
+      (IPC: imm_s.imm_psc_consistent GI sc),
     exists (GO: execution),
       ⟪WF': Wf GO ⟫ /\
-      ⟪ExecO: Oprogram_execution ProgO GO⟫ /\
+      ⟪ExecO: Oprogram_execution OCamlProgO GO⟫ /\
       ⟪OC: ocaml_consistent GO ⟫ /\
       ⟪SameBeh: same_behavior GO GI⟫.
-  Proof.
-    ins.
-    set (GO :=
-           {| acts := filterP (RW GI \₁ dom_rel (GI.(rmw))) GI.(acts);
-              lab := GI.(lab); (* should restrict domain *)
-              rmw := ∅₂;
-              (* same deps? *)
-              data := GI.(data);
-              addr := GI.(addr);
-              ctrl := GI.(ctrl);              
-              rmw_dep := ∅₂;
-              rf := GI.(rf) ⨾ ⦗set_compl (dom_rel GI.(rmw))⦘;
-              co := GI.(co) |}). 
-    exists GO. splits.
-    { destruct WF. 
-      split; subst GO; simpl; auto; admit. }
-    3: { red. splits; auto.
-         { admit. (* should convert to another graph *) }
-         { admit. }
-         { admit. }
-         { admit. }
-         { admit. }
-         { admit. }
-         subst GO. simpl. basic_solver. }
-    { red. splits.
-      { intros e EGOe.
-        right. 
-        (* destruct e; auto. right. *)
-        (* same threads, should be easy *) admit. }
-      intros thread subprog TP.
-      set (GOt := let eq_tid := (fun e => tid e = thread) in
-                  let restrict rel := ⦗eq_tid⦘ ⨾ rel ⨾ ⦗eq_tid⦘ in
-                  {| acts := filterP eq_tid GO.(acts);
-                     lab := GO.(lab); (* should restrict domain *)
-                     rmw := restrict GO.(rmw);
-                     data := restrict GO.(data);
-                     addr := restrict GO.(addr);
-                     ctrl := restrict GO.(ctrl);              
-                     rmw_dep := restrict GO.(rmw_dep);
-                     rf := restrict GO.(rf);
-                     co := restrict GI.(co) |}). 
-      exists GOt.
-      split.
-      2: { subst GOt. split; simpl; auto.
-           admit. (* E GO restriction; should be easy *)
-      }
-      (* ? show by induction that thread execution goes to some final state *)
-      red. 
-      admit. }
-
-    cut (ocaml_consistent GI).
-    { assert (RF': rf GO ≡ rf GI ⨾ ⦗set_compl (dom_rel (rmw GI))⦘).
-      { subst GO.  simpl. basic_solver. }
-      assert (E': E GO ≡₁ E GI ∩₁ (RW GI \₁ dom_rel (rmw GI))).
-      { subst GO. unfold acts_set. simpl.
-        red. split.
-        { red. ins. rewrite in_filterP_iff in H. red. desc. auto. }
-        red. ins. rewrite  in_filterP_iff. red in H. auto. }
-      assert (SB': sb GO ≡ ⦗RW GI \₁ dom_rel (rmw GI)⦘ ⨾ sb GI ⨾ ⦗RW GI \₁ dom_rel (rmw GI)⦘).
-      { unfold Execution.sb.        
-        rewrite !seqA. do 2 seq_rewrite <- id_inter.
-        rewrite set_interC. 
-        rewrite E'. 
-        basic_solver. }
-      assert (SC': Sc GO ≡₁ Sc GI) by intuition. 
-      assert (HBO': hbo GO ⊆ hbo GI).
-      { unfold OCaml.hb. apply clos_trans_mori.
-        apply union_mori; [rewrite SB'; basic_solver | ].
-        hahn_frame.
-        apply union_mori; [basic_solver | rewrite RF'; basic_solver]. }
-      assert (CO': co GO ≡ co GI) by intuition.
-      assert (FR': fr GO ≡ ⦗set_compl (dom_rel (rmw GI))⦘ ⨾ fr GI).
-      { unfold fr. rewrite CO'. rewrite <- seqA. apply seq_more; [| basic_solver].
-        subst GO. simpl. basic_solver. }
-      intros OCAML_GI. unfold ocaml_consistent. unfold ocaml_consistent in OCAML_GI.
-      splits; auto.
-      { red. rewrite E', RF'.
-        desc. red in Comp.
-        rewrite set_interC, <- set_interA.
-        rewrite set_inter_minus_r.
-        arewrite (R GO ∩₁ E GI ∩₁ RW GI ≡₁ R GO ∩₁ E GI) by basic_solver.
-        rewrite codom_eqv1.
-        rewrite set_minusE.
-        apply set_subset_inter; [rewrite set_interC; apply Comp | basic_solver]. }
-      { red. subst GO. simpl. rewrite inter_false_l. basic_solver. }
-      { rewrite HBO'. subst GO. simpl. desc. auto. }
-      { unfold fr. rewrite HBO'.
-        arewrite (rf GO ⊆ rf GI) by rewrite RF'; auto. 
-        subst GO. simpl. auto. desc. auto. }
-      
-      assert (W_RMW: W GI ⊆₁ RW GI \₁ dom_rel (rmw GI)).
-      { rewrite set_minusE.
-        apply set_subset_inter_r. split; [basic_solver| ].
-        sin_rewrite (WF.(wf_rmwD)).
-        rewrite dom_eqv1. rewrite set_compl_inter.
-        unionR left. type_solver. }
-      arewrite (rfe GO ⊆ rfe GI).
-      { unfold rfe. rewrite SB', RF'.
-        apply inclusion_minus_l.
-        rewrite rfi_union_rfe at 1. rewrite seq_union_l.
-        apply union_mori.        
-        { rewrite (WF.(wf_rfiD)). 
-          arewrite (rfi GI ⊆ sb GI).
-          apply seq_mori; [ | basic_solver]. 
-          apply eqv_rel_mori. apply W_RMW. }
-        unfold rfe. basic_solver. }
-      arewrite (fre GO ⊆ fre GI).
-      { unfold fre. rewrite SB', FR'.
-        apply inclusion_minus_l.
-        rewrite fri_union_fre at 1. rewrite seq_union_r.
-        apply union_mori.        
-        { rewrite (WF.(wf_friD)). 
-          arewrite (fri GI ⊆ sb GI).
-          rewrite <- seqA. 
-          apply seq_mori; [basic_solver |].
-          hahn_frame. apply eqv_rel_mori. apply W_RMW. }
-        unfold fre. basic_solver. }
-          
-      arewrite (coe GO ⊆ coe GI).
-      { unfold coe. rewrite SB', CO'. 
-        apply inclusion_minus_l.
-        rewrite coi_union_coe at 1. 
-        apply union_mori.        
-        { rewrite (WF.(wf_coiD)). 
-          arewrite (coi GI ⊆ sb GI).
-          apply seq_mori; hahn_frame; apply eqv_rel_mori; apply W_RMW. } 
-        unfold coe. basic_solver. }
-      rewrite SC'. 
-      arewrite (sb GO ⊆ sb GI) by rewrite SB'; basic_solver.
-      desc. auto. }
-    
-    (* need to specify location separation for OCaml program and prove that it's preserved in IMM program *)
-    assert (LSM: forall l,
-               (fun x => loc GI.(lab) x = Some l) \₁ is_init ⊆₁ ORlx GI \/
-               (fun x => loc GI.(lab) x = Some l) \₁ is_init ⊆₁ Sc GI) by admit.
-    assert (WSCFACQRMW : W GI ∩₁ Sc GI ≡₁ codom_rel (⦗F GI ∩₁ Acq GI⦘ ⨾ immediate (sb GI) ⨾ rmw GI)) by admit.
-    assert (RMWSC: rmw GI ≡ ⦗Sc GI⦘ ⨾ rmw GI ⨾ ⦗Sc GI⦘) by admit.
-    assert (WRLXF: W GI ∩₁ ORlx GI ⊆₁ codom_rel (⦗F GI ∩₁Acqrel GI⦘ ⨾ immediate (sb GI))) by admit. 
-    assert (RSCF: R GI ∩₁ Sc GI ⊆₁ codom_rel (⦗F GI ∩₁ Acq GI⦘ ⨾ immediate (sb GI))) by admit. 
-
-    apply (@imm_to_ocaml_consistent GI LSM WSCFACQRMW RMWSC WRLXF RSCF WF sc IPC).
-    (* goal on the shelf ? *)
-  Admitted.
+  Proof. Admitted.
   
   
 End OCamlMM_TO_IMM_S_PROG.
